cedar-lean/Cedar/Thm/SymCC/Opt.lean
@@ -19,6 +19,7 @@ import Cedar.SymCCOpt
 import Cedar.Thm.Data.Control
 import Cedar.Thm.Data.Set
 import Cedar.Thm.SymCC.Authorizer
+import Cedar.Thm.SymCC.Opt.AllowDeny
 import Cedar.Thm.SymCC.Opt.CompiledPolicies
 import Cedar.Thm.WellTypedVerification
 
@@ -92,6 +93,80 @@ theorem enforceCompiledPolicy_eqv_enforce_ok {p wp : Policy} {cp : CompiledPolic
 
 /--
 This theorem covers the "happy path" -- showing that if optimized policy
+compilation succeeds, then `enforce` and `enforcePairCompiledPolicies` are
+equivalent.
+-/
+theorem enforcePairCompiledPolicies_eqv_enforce_ok {ps₁ ps₂ wps₁ wps₂ : Policies} {cps₁ cps₂ : CompiledPolicies} {Γ : Validation.TypeEnv} :
+  CompiledPolicies.compile ps₁ Γ = .ok cps₁ →
+  CompiledPolicies.compile ps₂ Γ = .ok cps₂ →
+  wellTypedPolicies ps₁ Γ = .ok wps₁ →
+  wellTypedPolicies ps₂ Γ = .ok wps₂ →
+  enforce (wps₁.map Policy.toExpr ++ wps₂.map Policy.toExpr) (SymEnv.ofTypeEnv Γ) = enforcePairCompiledPolicies cps₁ cps₂
+:= by
+  simp [enforce, enforcePairCompiledPolicies]
+  intro hcps₁ hcps₂ hwps₁ hwps₂
+  simp [
+    cps_compile_produces_the_right_env hcps₁,
+    cps_compile_produces_the_right_env hcps₂,
+    cps_compile_produces_the_right_footprint hcps₁,
+    cps_compile_produces_the_right_footprint hcps₂,
+    cps_compile_produces_the_right_acyclicity hcps₁,
+    cps_compile_produces_the_right_acyclicity hcps₂,
+    compiled_policies_eq_wtps hcps₁ hwps₁,
+    compiled_policies_eq_wtps hcps₂ hwps₂,
+  ]
+  simp [footprints_append]
+  rw [Data.Set.make_make_eqv]
+  simp [List.Equiv, List.subset_def]
+  constructor
+  · intro t₁ h₁
+    cases h₁ <;> rename_i h₁
+    · replace ⟨t₂, h₁, htemp⟩ := h₁ ; subst t₁
+      simp [Data.Set.in_list_iff_in_set] at *
+      simp [footprints]
+      change t₂ ∈ _ ∪ _ at h₁
+      rw [Data.Set.mem_union_iff_mem_or] at h₁
+      cases h₁ <;> rename_i h₁
+      case' inl => left
+      case' inr => right ; left
+      all_goals {
+        simp [footprints] at h₁
+        rw [Data.Set.mem_mapUnion_iff_mem_exists] at h₁
+        replace ⟨x, h₁, h₂⟩ := h₁
+        simp [Data.Set.mem_map]
+        exists t₂
+        simp [Data.Set.mem_mapUnion_iff_mem_exists]
+        exists x
+        apply And.intro _ h₂
+        rw [List.mem_map] at h₁
+        exact h₁
+      }
+    · right ; right
+      simp [*]
+  · intro t₁ h₁
+    cases h₁ <;> rename_i h₁ <;> try (cases h₁ <;> rename_i h₁)
+    case right.inr.inr => right ; exact h₁
+    case' right.inl | right.inr.inl =>
+      left
+      simp [Data.Set.in_list_iff_in_set, Data.Set.mem_map] at h₁
+      replace ⟨t₂, h₁, htemp⟩ := h₁ ; subst t₁
+      simp [mem_footprints_iff] at h₁
+      replace ⟨x, ⟨p, hp, htemp⟩, h₁⟩ := h₁ ; subst x
+      exists t₂
+      simp [Data.Set.in_list_iff_in_set, HAppend.hAppend]
+      change t₂ ∈ _ ∪ _
+      rw [Data.Set.mem_union_iff_mem_or]
+    case' right.inl => left
+    case' right.inr.inl => right
+    all_goals {
+      simp [mem_footprints_iff]
+      exists p.toExpr
+      apply And.intro _ h₁
+      exists p
+    }
+
+/--
+This theorem covers the "happy path" -- showing that if optimized policy
 compilation succeeds, then `verifyEvaluate` and `verifyEvaluateOpt` are
 equivalent.
 -/
@@ -109,6 +184,28 @@ theorem verifyEvaluateOpt_eqv_verifyEvaluate_ok {p wp : Policy} {cp : CompiledPo
 
 /--
 This theorem covers the "happy path" -- showing that if optimized policy
+compilation succeeds, then `verifyIsAuthorized` and `verifyIsAuthorizedOpt` are
+equivalent.
+-/
+theorem verifyIsAuthorizedOpt_eqv_verifyIsAuthorized_ok {ps₁ ps₂ wps₁ wps₂ : Policies} {cps₁ cps₂ : CompiledPolicies} {Γ : Validation.TypeEnv} {φ : Term → Term → Term} :
+  CompiledPolicies.compile ps₁ Γ = .ok cps₁ →
+  CompiledPolicies.compile ps₂ Γ = .ok cps₂ →
+  wellTypedPolicies ps₁ Γ = .ok wps₁ →
+  wellTypedPolicies ps₂ Γ = .ok wps₂ →
+  verifyIsAuthorized φ wps₁ wps₂ (SymEnv.ofTypeEnv Γ) = .ok (verifyIsAuthorizedOpt φ cps₁ cps₂)
+:= by
+  simp [verifyIsAuthorized, verifyIsAuthorizedOpt]
+  simp [do_eq_ok]
+  intro hcps₁ hcps₂ hwps₁ hwps₂
+  simp [enforcePairCompiledPolicies_eqv_enforce_ok hcps₁ hcps₂ hwps₁ hwps₂]
+  have henvs : cps₁.εnv = cps₂.εnv := by
+    simp [cps_compile_produces_the_right_env hcps₁, cps_compile_produces_the_right_env hcps₂]
+  simp [henvs]
+  exists cps₁.term ; simp [cps_compile_produces_the_right_term hcps₁ hwps₁]
+  exists cps₂.term ; simp [cps_compile_produces_the_right_term hcps₂ hwps₂]
+
+/--
+This theorem covers the "happy path" -- showing that if optimized policy
 compilation succeeds, then `verifyNeverErrors` and `verifyNeverErrorsOpt` are
 equivalent.
 -/
@@ -119,6 +216,88 @@ theorem verifyNeverErrorsOpt_eqv_verifyNeverErrors_ok {p wp : Policy} {cp : Comp
 := by
   simp [verifyNeverErrors, verifyNeverErrorsOpt]
   exact verifyEvaluateOpt_eqv_verifyEvaluate_ok
+
+/--
+This theorem covers the "happy path" -- showing that if optimized policy
+compilation succeeds, then `verifyImplies` and `verifyImpliesOpt` are
+equivalent.
+-/
+theorem verifyImpliesOpt_eqv_verifyImplies_ok {ps₁ ps₂ wps₁ wps₂ : Policies} {cps₁ cps₂ : CompiledPolicies} {Γ : Validation.TypeEnv} :
+  CompiledPolicies.compile ps₁ Γ = .ok cps₁ →
+  CompiledPolicies.compile ps₂ Γ = .ok cps₂ →
+  wellTypedPolicies ps₁ Γ = .ok wps₁ →
+  wellTypedPolicies ps₂ Γ = .ok wps₂ →
+  verifyImplies wps₁ wps₂ (SymEnv.ofTypeEnv Γ) = .ok (verifyImpliesOpt cps₁ cps₂)
+:= by
+  simp [verifyImplies, verifyImpliesOpt]
+  exact verifyIsAuthorizedOpt_eqv_verifyIsAuthorized_ok
+
+/--
+This theorem covers the "happy path" -- showing that if optimized policy
+compilation succeeds, then `verifyAlwaysAllows` and `verifyAlwaysAllowsOpt` are
+equivalent.
+-/
+theorem verifyAlwaysAllowsOpt_eqv_verifyAlwaysAllows_ok {ps wps : Policies} {cps : CompiledPolicies} {Γ : Validation.TypeEnv} :
+  CompiledPolicies.compile ps Γ = .ok cps →
+  wellTypedPolicies ps Γ = .ok wps →
+  verifyAlwaysAllows wps (SymEnv.ofTypeEnv Γ) = .ok (verifyAlwaysAllowsOpt cps)
+:= by
+  simp [verifyAlwaysAllows, verifyAlwaysAllowsOpt]
+  intro hcps hwps
+  apply verifyImpliesOpt_eqv_verifyImplies_ok _ hcps (wellTypedPolicies_allowAll Γ) hwps
+  simp [CompiledPolicies.compile, Except.mapError, do_eq_ok]
+  simp [wellTypedPolicies_allowAll, isAuthorized_allowAll]
+  simp [CompiledPolicies.allowAll, cps_compile_produces_the_right_env hcps]
+  simp [footprints_singleton]
+
+/--
+This theorem covers the "happy path" -- showing that if optimized policy
+compilation succeeds, then `verifyAlwaysAllows` and `verifyAlwaysAllowsOpt` are
+equivalent.
+-/
+theorem verifyAlwaysDeniesOpt_eqv_verifyAlwaysDenies_ok {ps wps : Policies} {cps : CompiledPolicies} {Γ : Validation.TypeEnv} :
+  CompiledPolicies.compile ps Γ = .ok cps →
+  wellTypedPolicies ps Γ = .ok wps →
+  verifyAlwaysDenies wps (SymEnv.ofTypeEnv Γ) = .ok (verifyAlwaysDeniesOpt cps)
+:= by
+  simp [verifyAlwaysDenies, verifyAlwaysDeniesOpt]
+  intro hcps hwps
+  apply verifyImpliesOpt_eqv_verifyImplies_ok hcps _ hwps _ (ps₂ := [])
+  simp [CompiledPolicies.compile, Except.mapError, do_eq_ok]
+  simp [wellTypedPolicies_empty, isAuthorized_empty]
+  simp [CompiledPolicies.denyAll, cps_compile_produces_the_right_env hcps]
+  simp [footprints_empty, EmptyCollection.emptyCollection, Data.Set.map_empty]
+  simp [wellTypedPolicies_empty]
+
+/--
+This theorem covers the "happy path" -- showing that if optimized policy
+compilation succeeds, then `verifyEquivalent` and `verifyEquivalentOpt` are
+equivalent.
+-/
+theorem verifyEquivalentOpt_eqv_verifyEquivalent_ok {ps₁ ps₂ wps₁ wps₂ : Policies} {cps₁ cps₂ : CompiledPolicies} {Γ : Validation.TypeEnv} :
+  CompiledPolicies.compile ps₁ Γ = .ok cps₁ →
+  CompiledPolicies.compile ps₂ Γ = .ok cps₂ →
+  wellTypedPolicies ps₁ Γ = .ok wps₁ →
+  wellTypedPolicies ps₂ Γ = .ok wps₂ →
+  verifyEquivalent wps₁ wps₂ (SymEnv.ofTypeEnv Γ) = .ok (verifyEquivalentOpt cps₁ cps₂)
+:= by
+  simp [verifyEquivalent, verifyEquivalentOpt]
+  exact verifyIsAuthorizedOpt_eqv_verifyIsAuthorized_ok
+
+/--
+This theorem covers the "happy path" -- showing that if optimized policy
+compilation succeeds, then `verifyDisjoint` and `verifyDisjointOpt` are
+equivalent.
+-/
+theorem verifyDisjointOpt_eqv_verifyDisjoint_ok {ps₁ ps₂ wps₁ wps₂ : Policies} {cps₁ cps₂ : CompiledPolicies} {Γ : Validation.TypeEnv} :
+  CompiledPolicies.compile ps₁ Γ = .ok cps₁ →
+  CompiledPolicies.compile ps₂ Γ = .ok cps₂ →
+  wellTypedPolicies ps₁ Γ = .ok wps₁ →
+  wellTypedPolicies ps₂ Γ = .ok wps₂ →
+  verifyDisjoint wps₁ wps₂ (SymEnv.ofTypeEnv Γ) = .ok (verifyDisjointOpt cps₁ cps₂)
+:= by
+  simp [verifyDisjoint, verifyDisjointOpt]
+  exact verifyIsAuthorizedOpt_eqv_verifyIsAuthorized_ok
 
 /--
 If `CompiledPolicy.compile` succeeds, then `wellTypedPolicy` succeeds
@@ -132,6 +311,17 @@ theorem compile_ok_then_welltypedpolicy_ok {p : Policy} {Γ : Validation.TypeEnv
   cases h₀ : wellTypedPolicy p Γ <;> simp
 
 /--
+If `CompiledPolicies.compile` succeeds, then `wellTypedPolicies` succeeds
+-/
+theorem compile_ok_then_welltypedpolicies_ok (ps : Policies) {Γ : Validation.TypeEnv} :
+  Except.isOk (CompiledPolicies.compile ps Γ) →
+  Except.isOk (wellTypedPolicies ps Γ)
+:= by
+  simp [Except.isOk, Except.toBool]
+  simp [CompiledPolicies.compile, Except.mapError]
+  cases h₀ : wellTypedPolicies ps Γ <;> simp
+
+/--
 If `CompiledPolicy.compile` succeeds, then `wellTypedPolicy` succeeds
 -/
 theorem compile_ok_then_exists_wtp {p : Policy} {cp : CompiledPolicy} {Γ : Validation.TypeEnv} :
@@ -142,6 +332,21 @@ theorem compile_ok_then_exists_wtp {p : Policy} {cp : CompiledPolicy} {Γ : Vali
   have h₁ := compile_ok_then_welltypedpolicy_ok (by
     simp [Except.isOk_iff_exists]
     exists cp
+  )
+  simp [Except.isOk_iff_exists] at h₁
+  exact h₁
+
+/--
+If `CompiledPolicies.compile` succeeds, then `wellTypedPolicies` succeeds
+-/
+theorem compile_ok_then_exists_wtps {ps : Policies} {cps : CompiledPolicies} {Γ : Validation.TypeEnv} :
+  CompiledPolicies.compile ps Γ = .ok cps →
+  ∃ wps, wellTypedPolicies ps Γ = .ok wps
+:= by
+  intro h₀
+  have h₁ := compile_ok_then_welltypedpolicies_ok ps (by
+    simp [Except.isOk_iff_exists]
+    exists cps
   )
   simp [Except.isOk_iff_exists] at h₁
   exact h₁
@@ -168,4 +373,136 @@ theorem neverErrorsOpt?_eqv_neverErrors?_ok {p : Policy} {cp : CompiledPolicy} {
   simp [cp_compile_produces_the_right_env h₀]
   simp [compiled_policy_eq_wtp h₀ h₁]
   simp [verifyNeverErrorsOpt_eqv_verifyNeverErrors_ok h₀ h₁] at h₂
+  subst asserts ; rfl
+
+/--
+This theorem covers the "happy path" -- showing that if optimized policy
+compilation succeeds, then `wellTypedPolicies` succeeds and `implies?` and
+`impliesOpt?` are equivalent.
+-/
+theorem impliesOpt?_eqv_implies?_ok {ps₁ ps₂ : Policies} {cps₁ cps₂ : CompiledPolicies} {Γ : Validation.TypeEnv} :
+  Γ.WellFormed →
+  CompiledPolicies.compile ps₁ Γ = .ok cps₁ →
+  CompiledPolicies.compile ps₂ Γ = .ok cps₂ →
+  ∃ wps₁ wps₂,
+    wellTypedPolicies ps₁ Γ = .ok wps₁ ∧
+    wellTypedPolicies ps₂ Γ = .ok wps₂ ∧
+    impliesOpt? cps₁ cps₂ = implies? wps₁ wps₂ (SymEnv.ofTypeEnv Γ)
+:= by
+  simp [implies?, impliesOpt?]
+  simp [sat?]
+  intro hwf hcps₁ hcps₂
+  have ⟨wps₁, hwps₁⟩ := compile_ok_then_exists_wtps hcps₁
+  exists wps₁ ; apply And.intro hwps₁
+  have ⟨wps₂, hwps₂⟩ := compile_ok_then_exists_wtps hcps₂
+  exists wps₂ ; apply And.intro hwps₂
+  have ⟨asserts, h₁⟩ := verifyImplies_is_ok hwf hwps₁ hwps₂
+  simp [h₁]
+  simp [cps_compile_produces_the_right_env hcps₁]
+  simp [compiled_policies_eq_wtps hcps₁ hwps₁, compiled_policies_eq_wtps hcps₂ hwps₂]
+  simp [verifyImpliesOpt_eqv_verifyImplies_ok hcps₁ hcps₂ hwps₁ hwps₂] at h₁
+  subst asserts ; rfl
+
+/--
+This theorem covers the "happy path" -- showing that if optimized policy
+compilation succeeds, then `wellTypedPolicies` succeeds and `alwaysAllows?` and
+`alwaysAllowsOpt?` are equivalent.
+-/
+theorem alwaysAllowsOpt?_eqv_alwaysAllows?_ok {ps : Policies} {cps : CompiledPolicies} {Γ : Validation.TypeEnv} :
+  Γ.WellFormed →
+  CompiledPolicies.compile ps Γ = .ok cps →
+  ∃ wps,
+    wellTypedPolicies ps Γ = .ok wps ∧
+    alwaysAllowsOpt? cps = alwaysAllows? wps (SymEnv.ofTypeEnv Γ)
+:= by
+  simp [alwaysAllows?, alwaysAllowsOpt?]
+  simp [sat?]
+  intro hwf hcps
+  have ⟨wps, hwps⟩ := compile_ok_then_exists_wtps hcps
+  exists wps ; apply And.intro hwps
+  have ⟨asserts, h₁⟩ := verifyAlwaysAllows_is_ok hwf hwps
+  simp [h₁]
+  simp [cps_compile_produces_the_right_env hcps]
+  simp [compiled_policies_eq_wtps hcps hwps]
+  simp [verifyAlwaysAllowsOpt_eqv_verifyAlwaysAllows_ok hcps hwps] at h₁
+  subst asserts ; rfl
+
+/--
+This theorem covers the "happy path" -- showing that if optimized policy
+compilation succeeds, then `wellTypedPolicies` succeeds and `alwaysDenies?` and
+`alwaysDeniesOpt?` are equivalent.
+-/
+theorem alwaysDeniesOpt?_eqv_alwaysDenies?_ok {ps : Policies} {cps : CompiledPolicies} {Γ : Validation.TypeEnv} :
+  Γ.WellFormed →
+  CompiledPolicies.compile ps Γ = .ok cps →
+  ∃ wps,
+    wellTypedPolicies ps Γ = .ok wps ∧
+    alwaysDeniesOpt? cps = alwaysDenies? wps (SymEnv.ofTypeEnv Γ)
+:= by
+  simp [alwaysDenies?, alwaysDeniesOpt?]
+  simp [sat?]
+  intro hwf hcps
+  have ⟨wps, hwps⟩ := compile_ok_then_exists_wtps hcps
+  exists wps ; apply And.intro hwps
+  have ⟨asserts, h₁⟩ := verifyAlwaysDenies_is_ok hwf hwps
+  simp [h₁]
+  simp [cps_compile_produces_the_right_env hcps]
+  simp [compiled_policies_eq_wtps hcps hwps]
+  simp [verifyAlwaysDeniesOpt_eqv_verifyAlwaysDenies_ok hcps hwps] at h₁
+  subst asserts ; rfl
+
+/--
+This theorem covers the "happy path" -- showing that if optimized policy
+compilation succeeds, then `wellTypedPolicies` succeeds and `equivalent?` and
+`equivalentOpt?` are equivalent.
+-/
+theorem equivalent?_eqv_equivalentOpt?_ok {ps₁ ps₂ : Policies} {cps₁ cps₂ : CompiledPolicies} {Γ : Validation.TypeEnv} :
+  Γ.WellFormed →
+  CompiledPolicies.compile ps₁ Γ = .ok cps₁ →
+  CompiledPolicies.compile ps₂ Γ = .ok cps₂ →
+  ∃ wps₁ wps₂,
+    wellTypedPolicies ps₁ Γ = .ok wps₁ ∧
+    wellTypedPolicies ps₂ Γ = .ok wps₂ ∧
+    equivalentOpt? cps₁ cps₂ = equivalent? wps₁ wps₂ (SymEnv.ofTypeEnv Γ)
+:= by
+  simp [equivalent?, equivalentOpt?]
+  simp [sat?]
+  intro hwf hcps₁ hcps₂
+  have ⟨wps₁, hwps₁⟩ := compile_ok_then_exists_wtps hcps₁
+  exists wps₁ ; apply And.intro hwps₁
+  have ⟨wps₂, hwps₂⟩ := compile_ok_then_exists_wtps hcps₂
+  exists wps₂ ; apply And.intro hwps₂
+  have ⟨asserts, h₁⟩ := verifyEquivalent_is_ok hwf hwps₁ hwps₂
+  simp [h₁]
+  simp [cps_compile_produces_the_right_env hcps₁]
+  simp [compiled_policies_eq_wtps hcps₁ hwps₁, compiled_policies_eq_wtps hcps₂ hwps₂]
+  simp [verifyEquivalentOpt_eqv_verifyEquivalent_ok hcps₁ hcps₂ hwps₁ hwps₂] at h₁
+  subst asserts ; rfl
+
+/--
+This theorem covers the "happy path" -- showing that if optimized policy
+compilation succeeds, then `wellTypedPolicies` succeeds and `disjoint?` and
+`disjointOpt?` are equivalent.
+-/
+theorem disjoint?_eqv_disjointOpt?_ok {ps₁ ps₂ : Policies} {cps₁ cps₂ : CompiledPolicies} {Γ : Validation.TypeEnv} :
+  Γ.WellFormed →
+  CompiledPolicies.compile ps₁ Γ = .ok cps₁ →
+  CompiledPolicies.compile ps₂ Γ = .ok cps₂ →
+  ∃ wps₁ wps₂,
+    wellTypedPolicies ps₁ Γ = .ok wps₁ ∧
+    wellTypedPolicies ps₂ Γ = .ok wps₂ ∧
+    disjointOpt? cps₁ cps₂ = disjoint? wps₁ wps₂ (SymEnv.ofTypeEnv Γ)
+:= by
+  simp [disjoint?, disjointOpt?]
+  simp [sat?]
+  intro hwf hcps₁ hcps₂
+  have ⟨wps₁, hwps₁⟩ := compile_ok_then_exists_wtps hcps₁
+  exists wps₁ ; apply And.intro hwps₁
+  have ⟨wps₂, hwps₂⟩ := compile_ok_then_exists_wtps hcps₂
+  exists wps₂ ; apply And.intro hwps₂
+  have ⟨asserts, h₁⟩ := verifyDisjoint_is_ok hwf hwps₁ hwps₂
+  simp [h₁]
+  simp [cps_compile_produces_the_right_env hcps₁]
+  simp [compiled_policies_eq_wtps hcps₁ hwps₁, compiled_policies_eq_wtps hcps₂ hwps₂]
+  simp [verifyDisjointOpt_eqv_verifyDisjoint_ok hcps₁ hcps₂ hwps₁ hwps₂] at h₁
   subst asserts ; rfl
