cedar-lean/Cedar/Thm/SymCC/Opt/AllowDeny.lean
@@ -1,0 +1,70 @@
+/-
+ Copyright Cedar Contributors
+
+ Licensed under the Apache License, Version 2.0 (the "License");
+ you may not use this file except in compliance with the License.
+ You may obtain a copy of the License at
+
+      https://www.apache.org/licenses/LICENSE-2.0
+
+ Unless required by applicable law or agreed to in writing, software
+ distributed under the License is distributed on an "AS IS" BASIS,
+ WITHOUT WARRANTIES OR CONDITIONS OF ANY KIND, either express or implied.
+ See the License for the specific language governing permissions and
+ limitations under the License.
+-/
+
+import Cedar.SymCC
+
+/-!
+Proofs about various functions applied to `allowAll` and `denyAll` policies, and empty policy sets.
+-/
+
+namespace Cedar.Thm
+
+open Cedar.Spec Cedar.SymCC
+
+/--
+`wellTypedPolicies` on the empty policy set
+-/
+theorem wellTypedPolicies_empty (Γ : Validation.TypeEnv) :
+  wellTypedPolicies [] Γ = .ok []
+:= by
+  simp [wellTypedPolicies, pure, Except.pure]
+
+/--
+`wellTypedPolicies` on `Policy.allowAll`
+-/
+theorem wellTypedPolicies_allowAll (Γ : Validation.TypeEnv) :
+  wellTypedPolicies [Policy.allowAll] Γ = .ok [verifyAlwaysAllows.allowAll]
+:= by
+  simp [wellTypedPolicies, wellTypedPolicy]
+  simp [Validation.typecheckPolicy, Policy.allowAll, verifyAlwaysAllows.allowAll]
+  simp [Policy.toExpr, PrincipalScope.toExpr, ActionScope.toExpr, ResourceScope.toExpr, Scope.toExpr, Conditions.toExpr]
+  simp [Validation.typeOf, Validation.substituteAction, Validation.mapOnVars, Validation.typeOfLit, Validation.ok, Validation.typeOfAnd, Validation.TypedExpr.typeOf, Validation.TypedExpr.toExpr, Validation.subty, Validation.lub?, Validation.lubBool]
+
+/--
+`SymCC.isAuthorized` on the empty policy set
+-/
+theorem isAuthorized_empty (εnv : SymEnv) :
+  SymCC.isAuthorized [] εnv = .ok (.bool false)
+:= by
+  simp [SymCC.isAuthorized, SymCC.satisfiedPolicies]
+  simp [
+    Factory.and, Factory.or, Factory.not, Factory.anyTrue, Factory.eq, Factory.eq.simplify,
+    Factory.someOf, Term.typeOf, TermPrim.typeOf
+  ]
+
+/--
+`SymCC.isAuthorized` on `verifyAlwaysAllows.allowAll`
+-/
+theorem isAuthorized_allowAll (εnv : SymEnv) :
+  SymCC.isAuthorized [verifyAlwaysAllows.allowAll] εnv = .ok (.bool true)
+:= by
+  simp [verifyAlwaysAllows.allowAll, SymCC.isAuthorized, SymCC.satisfiedPolicies, compileWithEffect]
+  simp [Policy.toExpr, PrincipalScope.toExpr, ActionScope.toExpr, ResourceScope.toExpr, Scope.toExpr, Conditions.toExpr, Condition.toExpr]
+  simp [compile, compilePrim, compileAnd]
+  simp [
+    Factory.and, Factory.or, Factory.not, Factory.anyTrue, Factory.eq, Factory.eq.simplify, Factory.ite, Factory.ite.simplify,
+    Factory.someOf, Factory.noneOf, Factory.ifSome, Factory.isNone, Factory.option.get, Term.typeOf, TermPrim.typeOf
+  ]
